arm+arm-hyp+aarch64 machine: SGI interface
Define the new constants numSGIs and gicNumTargets, plus a new
machine operation ipiSendTarget.

Signed-off-by: Gerwin Klein <gerwin.klein@proofcraft.systems>

spec/machine/ARM_HYP/Platform.thy
@@ -32,10 +32,38 @@ section \<open>Platform Constants\<close>
 
 context Arch begin global_naming ARM_HYP
 
+(* General interrupts *)
 value_type irq_len = Kernel_Config.irqBits (* IRQ_CNODE_SLOT_BITS *)
 type_synonym irq = "irq_len word"
-type_synonym paddr = word32
 
+(* Software-generated interrupts *)
+definition numSGIs_bits :: nat where
+  "numSGIs_bits = 4"
+
+definition numSGIs :: nat where
+  "numSGIs = 2^numSGIs_bits"
+
+definition gicNumTargets_bits :: nat where
+  "gicNumTargets_bits \<equiv> if Kernel_Config.config_ARM_GIC_V3 then 5 else 3"
+
+definition gicNumTargets :: nat where
+  "gicNumTargets \<equiv> 2^gicNumTargets_bits"
+
+end
+
+(* Need to declare code equation outside Arch locale. Used in value_type below. *)
+lemmas [code] = ARM_HYP.numSGIs_bits_def ARM_HYP.gicNumTargets_bits_def
+
+context Arch begin global_naming ARM_HYP
+
+value_type sgi_irq_len = numSGIs_bits
+type_synonym sgi_irq = "sgi_irq_len word"
+
+value_type sgi_target_len = gicNumTargets_bits
+type_synonym sgi_target = "sgi_target_len word"
+
+(* Physical addresses *)
+type_synonym paddr = machine_word
 abbreviation (input) "toPAddr \<equiv> id"
 abbreviation (input) "fromPAddr \<equiv> id"
 
